所以
\[ \int_{a}^{\frac{a+b}{2}}|f(x)f'(x)|\,\mathrm{d}x \leq \frac{1}{2}g^{2}\left(\frac{a+b}{2}\right) \]
及
\[ \int_{\frac{a+b}{2}}^{b}|f(x)f'(x)|\,\mathrm{d}x \leq \frac{1}{2}h^{2}\left(\frac{a+b}{2}\right). \]

再由柯西—施瓦兹不等式，可得：
\[ 
\begin{aligned} 
g^{2}\left(\frac{a+b}{2}\right) &= \left(\int_{a}^{\frac{a+b}{2}}|f'(t)|\,\mathrm{d}t\right)^{2} \\ 
&\leq \left(\int_{a}^{\frac{a+b}{2}}1^{2}\,\mathrm{d}t\right)\left(\int_{a}^{\frac{a+b}{2}}|f'(t)|^{2}\,\mathrm{d}t\right) = \frac{b-a}{2}\int_{a}^{\frac{a+b}{2}}|f'(t)|^{2}\,\mathrm{d}t 
\end{aligned} 
\]
以及
\[ 
\begin{aligned} 
h^{2}\left(\frac{a+b}{2}\right) &= \left(\int_{\frac{a+b}{2}}^{b}|f'(t)|\,\mathrm{d}t\right)^{2} \\ 
&\leq \left(\int_{\frac{a+b}{2}}^{b}1^{2}\,\mathrm{d}t\right)\left(\int_{\frac{a+b}{2}}^{b}|f'(t)|^{2}\,\mathrm{d}t\right) = \frac{b-a}{2}\int_{\frac{a+b}{2}}^{b}|f'(t)|^{2}\,\mathrm{d}t 
\end{aligned} 
\]

因此
\[ 
\begin{aligned} 
\int_{a}^{b}|f(x)f'(x)|\,\mathrm{d}x &= \int_{a}^{\frac{a+b}{2}}|f(x)f'(x)|\,\mathrm{d}x + \int_{\frac{a+b}{2}}^{b}|f(x)f'(x)|\,\mathrm{d}x \\ 
&\leq \frac{1}{2}g^{2}\left(\frac{a+b}{2}\right) + \frac{1}{2}h^{2}\left(\frac{a+b}{2}\right) \\ 
&\leq \frac{b-a}{4}\int_{a}^{\frac{a+b}{2}}|f'(t)|^{2}\,\mathrm{d}t + \frac{b-a}{4}\int_{\frac{a+b}{2}}^{b}|f'(t)|^{2}\,\mathrm{d}t \\ 
&= \frac{b-a}{4}\int_{a}^{b}|f'(x)|^{2}\,\mathrm{d}x 
\end{aligned} 
\]

即
\[ \int_{a}^{b}|f(x)f'(x)|\,\mathrm{d}x \leq \frac{b-a}{4}\int_{a}^{b}|f'(x)|^{2}\,\mathrm{d}x, \]

取 \(a=0, b=2\) 可得：
\[ \int_{0}^{2}|f(x)f'(x)|\,\mathrm{d}x \leq \frac{1}{2}\int_{0}^{2}|f'(x)|^{2}\,\mathrm{d}x \leq \int_{0}^{2}|f'(x)|^{2}\,\mathrm{d}x. \]

即证出：
\[ \int_{0}^{2}|f(x)f'(x)|\,\mathrm{d}x \leq \int_{0}^{2}|f'(x)|^{2}\,\mathrm{d}x. \]

1.【参考解答】：令 \(g(x) = \sum_{n=0}^{\infty}\frac{1}{n!}x^{n+2}\)，其中 \(x \in (-\infty, +\infty)\)，则利用幂级数的连续可微性可知：